\documentclass{article}
\usepackage{graphicx}
\begin{document}

\begin{center}

\section*{Task}
{\Large$S\ K\ K = I$ proof}\\

\section*{Solution}
    
{\Large$(\lambda x.\lambda y.\lambda z.(x\ z)\ (y\ z)) (\lambda x.\lambda y.x)\ (\lambda x.\lambda y.x)$\\
$\rightarrow_\beta\ (\lambda y.\lambda z.((\lambda x.\lambda y.x)\ z)\ (y\ z)) (\lambda x.\lambda y.x)$\\
$\rightarrow_\beta\ (\lambda z.((\lambda x.\lambda y.x)\ z))\ ((\lambda x.\lambda y.x)\ z)$\\
$\rightarrow_\beta\ (\lambda z.((\lambda x.\lambda y.x)\ z))\ z)$\\
$\rightarrow_\beta\ (\lambda z.z)$\\
$\equiv I$}

\end{center}

\end{document}